Split out biabduction

Flow.v
@@ -8,100 +8,61 @@ Local Open Scope string_scope.
 Local Open Scope Z_scope.
 Local Open Scope list_scope.
 
-Module Biabduction.
+Definition val := Z.
 
-  (* like the member predicate. or modulo equivalence? *)
-  Inductive split : assertion -> assertion -> assertion -> Prop :=
-    | split_one : forall h2 x y,
-      split (pts x y ** h2) (pts x y) h2
-
-    | split_next : forall h2 x y h h1,
-      split h1 h h2 ->
-      split (pts x y ** h2) h h2
+Inductive expr : Type :=
+  | pvar (x: ident)
+  | pconst (n: val)
+  | plet (x: ident) (e1: expr) (e2: expr)
+  (* | pref (x: ident) *)
+  (* | pderef (x: ident) *)
+  (* | passign (x1: ident) (x2: ident) *)
+  | pif (x: ident) (e1: expr) (e2: expr)
+  | pcall (x: ident) (a: ident)
   .
 
-  Inductive biab : assertion -> assertion -> assertion -> Prop :=
+Inductive eresult : Type :=
+  | enorm : val -> eresult
+.
 
-    | biab_base : forall s m,
-      biab s m (pure True)
+Reserved Notation " 'eval[' s ',' h ',' e ']' '=>' '[' s1 ',' h1 ',' r ']' " (at level 50, left associativity).
 
-    | biab_missing : forall x y a m,
-      biab emp ((pts x y) ** m) ((pts x y) ** a)
+Definition store := store Z.
 
-    | biab_match : forall x y z a b m m1,
-      biab b m a ->
-      (z = y) //\\ m = m1 ->
-      biab ((pts x z) ** b) m1 ((pts x y) ** a)
-  .
+Inductive bigstep : store -> heap -> expr -> store -> heap -> eresult -> Prop :=
+  | eval_pvar : forall s h x v,
+    Some v = s x ->
+    eval[ s, h, pvar x ]=>[ s, h, enorm v]
+  | eval_pconst : forall s h x,
+    eval[ s, h, pconst x ] => [ s, h, enorm x]
+  | eval_plet : forall x e1 e2 v s h h2 s2 s1 h1 r,
+    eval[ s, h, e1 ] => [ s1, h1, enorm v] ->
+    eval[ supdate x v s1, h1, e2 ] => [ s2, h2, r] ->
+    eval[ s, h, plet x e1 e2 ] => [ s2, h2, r ]
+  (* | eval_pref : forall x s (h:heap) l,
+    h l = None ->
+    eval[ s, h, pref x ] => [ s, hupdate l (s x) h, enorm l]
+  | eval_deref : forall x s (h:heap) v,
+    h (s x) = Some v ->
+    eval[ s, h, pderef x ] => [ s, h, enorm v]
+  | eval_assign : forall x1 x2 s h,
+    eval[ s, h, passign x1 x2 ] => [ s, hupdate (s x1) (s x2) h, enorm 0] *)
 
-  Example ex1 : forall x y a b,
-    biab (pts x y ** emp) (pts a b) (pts x y ** pts a b).
+  where " 'eval[' s ',' h ',' e ']' '=>' '[' s1 ',' h1 ',' r ']' " := (bigstep s h e s1 h1 r)
+.
+
+Module ProgramExamples.
+
+  (* Example ex_ref :
+    eval[ sempty, hempty, plet "x" (pconst 1) (pref "x") ]=>[ sempty, hupdate 2 1 hempty, enorm 2 ].
   Proof.
-    intros.
-    apply biab_match with (m := pts a b).
-    (* apply biab_missing with (m := pts a b). *)
+    apply eval_plet with (v:=1) (s1:=sempty) (s2:=supdate "x" 1 sempty) (h1:=hempty).
+    apply eval_pconst.
+    apply eval_pref.
+    constructor.
+  Qed. *)
 
-  Admitted.
-
-End Biabduction.
-
-Module Flow3.
-
-  Definition val := Z.
-
-  Inductive expr : Type :=
-    | pvar (x: ident)
-    | pconst (n: val)
-    | plet (x: ident) (e1: expr) (e2: expr)
-    (* | pref (x: ident) *)
-    (* | pderef (x: ident) *)
-    (* | passign (x1: ident) (x2: ident) *)
-    | pif (x: ident) (e1: expr) (e2: expr)
-    | pcall (x: ident) (a: ident)
-    .
-
-  Inductive eresult : Type :=
-    | enorm : val -> eresult
-  .
-
-  Reserved Notation " 'eval[' s ',' h ',' e ']' '=>' '[' s1 ',' h1 ',' r ']' " (at level 50, left associativity).
-
-  Definition store := store Z.
-
-  Inductive bigstep : store -> heap -> expr -> store -> heap -> eresult -> Prop :=
-    | eval_pvar : forall s h x v,
-      Some v = s x ->
-      eval[ s, h, pvar x ]=>[ s, h, enorm v]
-    | eval_pconst : forall s h x,
-      eval[ s, h, pconst x ] => [ s, h, enorm x]
-    | eval_plet : forall x e1 e2 v s h h2 s2 s1 h1 r,
-      eval[ s, h, e1 ] => [ s1, h1, enorm v] ->
-      eval[ supdate x v s1, h1, e2 ] => [ s2, h2, r] ->
-      eval[ s, h, plet x e1 e2 ] => [ s2, h2, r ]
-    (* | eval_pref : forall x s (h:heap) l,
-      h l = None ->
-      eval[ s, h, pref x ] => [ s, hupdate l (s x) h, enorm l]
-    | eval_deref : forall x s (h:heap) v,
-      h (s x) = Some v ->
-      eval[ s, h, pderef x ] => [ s, h, enorm v]
-    | eval_assign : forall x1 x2 s h,
-      eval[ s, h, passign x1 x2 ] => [ s, hupdate (s x1) (s x2) h, enorm 0] *)
-
-    where " 'eval[' s ',' h ',' e ']' '=>' '[' s1 ',' h1 ',' r ']' " := (bigstep s h e s1 h1 r)
-  .
-
-  Module ProgramExamples.
-
-    (* Example ex_ref :
-      eval[ sempty, hempty, plet "x" (pconst 1) (pref "x") ]=>[ sempty, hupdate 2 1 hempty, enorm 2 ].
-    Proof.
-      apply eval_plet with (v:=1) (s1:=sempty) (s2:=supdate "x" 1 sempty) (h1:=hempty).
-      apply eval_pconst.
-      apply eval_pref.
-      constructor.
-    Qed. *)
-
-  End ProgramExamples.
+End ProgramExamples.
 
 Definition precond := assertion.
 Definition postcond := Z -> assertion.
@@ -109,343 +70,343 @@ Definition postcond := Z -> assertion.
 
 Module StagesDeep.
 
-  Inductive stages : Type :=
-    | req : precond -> stages
-    | ens : postcond -> stages
-    | seq : stages -> stages -> stages
-    (* | fexists : (Z -> stages) -> stages. *)
-    | fexists : ident -> stages -> stages.
+Inductive stages : Type :=
+  | req : precond -> stages
+  | ens : postcond -> stages
+  | seq : stages -> stages -> stages
+  (* | fexists : (Z -> stages) -> stages. *)
+  | fexists : ident -> stages -> stages.
 
-  Definition flow := Z -> stages.
+Definition flow := Z -> stages.
 
-  Infix ";;" := seq (at level 80, right associativity).
+Infix ";;" := seq (at level 80, right associativity).
 
-  (* Fixpoint replace_ret x f :=
-    match f with
-    | ens q => ens (fun r s h => ((r = s x) //\\ q (s x)) s h)
-    | req p => f
-    | seq a b => seq a (replace_ret x b)
-    | fexists i f => fexists i (replace_ret x f)
-    end. *)
+(* Fixpoint replace_ret x f :=
+  match f with
+  | ens q => ens (fun r s h => ((r = s x) //\\ q (s x)) s h)
+  | req p => f
+  | seq a b => seq a (replace_ret x b)
+  | fexists i f => fexists i (replace_ret x f)
+  end. *)
 
-  Inductive result : Type :=
-  | norm : Z -> result
-  .
+Inductive result : Type :=
+| norm : Z -> result
+.
 
-  Reserved Notation " 'sem[' t ',' s ',' h ']=>[' t1 ',' s1 ',' h1 ',' r ']' '|=' f " (at level 50, left associativity).
+Reserved Notation " 'sem[' t ',' s ',' h ']=>[' t1 ',' s1 ',' h1 ',' r ']' '|=' f " (at level 50, left associativity).
 
-  (* axiomatization of semantics for staged formulae *)
-  Inductive satisfies : bool -> store -> heap -> bool -> store -> heap -> result -> flow -> Prop :=
-    | sem_req: forall h3 p s1 s2 h1 r r1 f,
-      (exists h2, h3 = hunion h1 h2 /\ hdisjoint h1 h2 /\ p s1 h2) ->
-      f r1 = req p ->
-      sem[true, s1, h3]=>[true, s2, h1, norm r] |= f
-    | sem_ens: forall h1 h3 q v s f,
-      (exists h2, h3 = hunion h1 h2 /\ hdisjoint h1 h2 /\ q v s h2) ->
-      (* f r1 = ens ((r1 = v) //\\ q) -> *)
-      f v = ens q ->
-      sem[true, s, h1]=>[true, s, h3, norm v] |= f
-    | sem_ex: forall s s1 h1 h2 x e r,
-      (* the reason we can't use hoas is that the binding to the existential has to appear in the stack... *)
-      (exists v, sem[true, supdate x v s, h1]=>[true, s1, h2, r] |= e) ->
-      sem[true, s, h1]=>[true, s1, h2, r] |= fun r1 => fexists x (e r1)
-    | sem_seq: forall f1 f2 r1 h1 h2 h3 c s1 s2 s3 r2 st1 st2 ff,
-      sem[true, s1, h1]=>[true, s2, h2, norm r1] |= f1 ->
-      sem[true, s2, h2]=>[c, s3, h3, r2] |= f2 ->
-      st1 = f1 r1 ->
-      st2 = f2 r1 ->
-      ff r1 = (st1;;st2) ->
-      sem[true, s1, h1]=>[c, s3, h3, r2] |= ff
+(* axiomatization of semantics for staged formulae *)
+Inductive satisfies : bool -> store -> heap -> bool -> store -> heap -> result -> flow -> Prop :=
+  | sem_req: forall h3 p s1 s2 h1 r r1 f,
+    (exists h2, h3 = hunion h1 h2 /\ hdisjoint h1 h2 /\ p s1 h2) ->
+    f r1 = req p ->
+    sem[true, s1, h3]=>[true, s2, h1, norm r] |= f
+  | sem_ens: forall h1 h3 q v s f,
+    (exists h2, h3 = hunion h1 h2 /\ hdisjoint h1 h2 /\ q v s h2) ->
+    (* f r1 = ens ((r1 = v) //\\ q) -> *)
+    f v = ens q ->
+    sem[true, s, h1]=>[true, s, h3, norm v] |= f
+  | sem_ex: forall s s1 h1 h2 x e r,
+    (* the reason we can't use hoas is that the binding to the existential has to appear in the stack... *)
+    (exists v, sem[true, supdate x v s, h1]=>[true, s1, h2, r] |= e) ->
+    sem[true, s, h1]=>[true, s1, h2, r] |= fun r1 => fexists x (e r1)
+  | sem_seq: forall f1 f2 r1 h1 h2 h3 c s1 s2 s3 r2 st1 st2 ff,
+    sem[true, s1, h1]=>[true, s2, h2, norm r1] |= f1 ->
+    sem[true, s2, h2]=>[c, s3, h3, r2] |= f2 ->
+    st1 = f1 r1 ->
+    st2 = f2 r1 ->
+    ff r1 = (st1;;st2) ->
+    sem[true, s1, h1]=>[c, s3, h3, r2] |= ff
 
-  where " 'sem[' t ',' s ',' h ']=>[' t1 ',' s1 ',' h1 ',' r ']' '|=' f " := (satisfies t s h t1 s1 h1 r f)
-  .
+where " 'sem[' t ',' s ',' h ']=>[' t1 ',' s1 ',' h1 ',' r ']' '|=' f " := (satisfies t s h t1 s1 h1 r f)
+.
 
-  Module SemanticsExamples.
+Module SemanticsExamples.
 
-    Definition f1 : flow := fun r => ens (fun r1 => pure (r1=1 /\ r=r1)).
-    Definition f2 : flow := fun (r:Z) => req (fun s h => s "x" = Some 1).
+  Definition f1 : flow := fun r => ens (fun r1 => pure (r1=1 /\ r=r1)).
+  Definition f2 : flow := fun (r:Z) => req (fun s h => s "x" = Some 1).
 
-    (* ex z; req x->z; ens[r] x->1/\r=1 *)
-    Definition f3 : flow := fun r =>
-      (* fexists "z" (req (pts "x" "z") ;; ens ((r=1) //\\ ptsval "x" 1)). *)
-      fexists "z" (req (pts "x" "z") ;; ens (fun r1 => (r=r1) //\\ ptsval "x" 1)).
+  (* ex z; req x->z; ens[r] x->1/\r=1 *)
+  Definition f3 : flow := fun r =>
+    (* fexists "z" (req (pts "x" "z") ;; ens ((r=1) //\\ ptsval "x" 1)). *)
+    fexists "z" (req (pts "x" "z") ;; ens (fun r1 => (r=r1) //\\ ptsval "x" 1)).
 
-    Example ex_sem_f1:
-      sem[true, sempty, hempty]=>[true, sempty, hempty, norm(1)] |= f1.
-    Proof.
-      apply sem_ens with (q := fun r => pure (r=1)).
-      exists hempty.
-      heap.
-      unfold pure.
-      intuition auto.
-      unfold f1.
-      f_equal.
-      unfold pure.
-      apply functional_extensionality.
-      intros.
-      apply functional_extensionality.
-      intros.
-      apply functional_extensionality.
-      intros.
-      auto.
-      apply propositional_extensionality.
-      intuition auto.
-    Qed.
+  Example ex_sem_f1:
+    sem[true, sempty, hempty]=>[true, sempty, hempty, norm(1)] |= f1.
+  Proof.
+    apply sem_ens with (q := fun r => pure (r=1)).
+    exists hempty.
+    heap.
+    unfold pure.
+    intuition auto.
+    unfold f1.
+    f_equal.
+    unfold pure.
+    apply functional_extensionality.
+    intros.
+    apply functional_extensionality.
+    intros.
+    apply functional_extensionality.
+    intros.
+    auto.
+    apply propositional_extensionality.
+    intuition auto.
+  Qed.
 
-    (* Example ex_sem_f3:
-      sem[true, (supdate "x" 2 sempty), (hupdate 2 3 hempty) ]=>[
-        true, (supdate "x" 2 sempty), (hupdate 2 1 hempty), norm(1)] |= f3.
-    Proof.
-    (* unfold f3. *)
-      apply sem_ex.
-      exists 1.
-    (* Unset Printing Notations. *)
-      apply sem_seq with (f1 := fun r => req (pts "x" "z"))
-        (f2 := fun r => ens (ptsval "x" 1))
-        (r1 := 1)
-        (h2 := hempty)
-        (s2 := (supdate "x" 2 sempty))
-      .
-      - apply sem_req.
-      exists (hupdate 2 3 hempty).
-      heap.
-      unfold pts.
-      unfold contains.
-      unfold supdate. simpl.
-      admit.
-      -
-      unfold pureconj.
-      apply sem_ens.
-      admit.
-      - auto.
-    Admitted. *)
-    (* Qed. *)
+  (* Example ex_sem_f3:
+    sem[true, (supdate "x" 2 sempty), (hupdate 2 3 hempty) ]=>[
+      true, (supdate "x" 2 sempty), (hupdate 2 1 hempty), norm(1)] |= f3.
+  Proof.
+  (* unfold f3. *)
+    apply sem_ex.
+    exists 1.
+  (* Unset Printing Notations. *)
+    apply sem_seq with (f1 := fun r => req (pts "x" "z"))
+      (f2 := fun r => ens (ptsval "x" 1))
+      (r1 := 1)
+      (h2 := hempty)
+      (s2 := (supdate "x" 2 sempty))
+    .
+    - apply sem_req.
+    exists (hupdate 2 3 hempty).
+    heap.
+    unfold pts.
+    unfold contains.
+    unfold supdate. simpl.
+    admit.
+    -
+    unfold pureconj.
+    apply sem_ens.
+    admit.
+    - auto.
+  Admitted. *)
+  (* Qed. *)
 
-  End SemanticsExamples.
+End SemanticsExamples.
 
 End StagesDeep.
 
 (* Module StagesShallow. *)
 
-  Inductive result : Type :=
-    | norm : Z -> result.
+Inductive result : Type :=
+  | norm : Z -> result.
 
-  Definition flow := bool -> store -> heap -> bool -> store -> heap -> result -> Prop.
+Definition flow := bool -> store -> heap -> bool -> store -> heap -> result -> Prop.
 
-  Definition req : precond -> flow := fun p c1 s1 h1 c2 s2 h2 r =>
-    c1 = true /\ c2 = true /\
-    s1 = s2 /\
-    (* h3 is the piece taken out satisfying p *)
-    exists h3, h1 = hunion h2 h3 /\ hdisjoint h2 h3 /\ p s1 h3.
-    (* TODO only true case for now *)
+Definition req : precond -> flow := fun p c1 s1 h1 c2 s2 h2 r =>
+  c1 = true /\ c2 = true /\
+  s1 = s2 /\
+  (* h3 is the piece taken out satisfying p *)
+  exists h3, h1 = hunion h2 h3 /\ hdisjoint h2 h3 /\ p s1 h3.
+  (* TODO only true case for now *)
 
-  Definition ens : postcond -> flow := fun q c1 s1 h1 c2 s2 h2 r =>
-    c1 = true /\ c2 = true /\
-    s1 = s2 /\
-    (* forall v, r = norm v -> *)
-    exists v, r = norm v /\
-    (* h3 is the piece satisfying q that is addded to h1 *)
-      exists h3, h2 = hunion h1 h3 /\ hdisjoint h1 h3 /\ q v s1 h3.
+Definition ens : postcond -> flow := fun q c1 s1 h1 c2 s2 h2 r =>
+  c1 = true /\ c2 = true /\
+  s1 = s2 /\
+  (* forall v, r = norm v -> *)
+  exists v, r = norm v /\
+  (* h3 is the piece satisfying q that is addded to h1 *)
+    exists h3, h2 = hunion h1 h3 /\ hdisjoint h1 h3 /\ q v s1 h3.
 
-  Definition seq : flow -> flow -> flow := fun f1 f2 c1 s1 h1 c2 s2 h2 r =>
-    c1 = true /\ c2 = true /\
-    exists s3 h3 r1,
-    f1 c1 s1 h1 true s3 h3 r1 /\
-    f2 true s3 h3 c2 s2 h2 r.
+Definition seq : flow -> flow -> flow := fun f1 f2 c1 s1 h1 c2 s2 h2 r =>
+  c1 = true /\ c2 = true /\
+  exists s3 h3 r1,
+  f1 c1 s1 h1 true s3 h3 r1 /\
+  f2 true s3 h3 c2 s2 h2 r.
 
-  Infix ";;" := seq (at level 80, right associativity).
+Infix ";;" := seq (at level 80, right associativity).
 
-  (* we can't use hoas for this as the existential binding has to appear in the stack *)
-  Definition fexists : ident -> flow -> flow := fun i f c1 s1 h1 c2 s2 h2 r =>
-    c1 = true /\ c2 = true /\
-    s1 i = None /\
-    exists v,
-      f c1 (supdate i v s1) h1 c2 s2 h2 r.
+(* we can't use hoas for this as the existential binding has to appear in the stack *)
+Definition fexists : ident -> flow -> flow := fun i f c1 s1 h1 c2 s2 h2 r =>
+  c1 = true /\ c2 = true /\
+  s1 i = None /\
+  exists v,
+    f c1 (supdate i v s1) h1 c2 s2 h2 r.
 
-  Definition replace_ret (x:ident) (f:flow) : flow := fun c1 s1 h1 c2 s2 h2 r =>
-    exists v, Some v = s1 x /\
-    f c1 s1 h1 c2 s2 h2 (norm v).
+Definition replace_ret (x:ident) (f:flow) : flow := fun c1 s1 h1 c2 s2 h2 r =>
+  exists v, Some v = s1 x /\
+  f c1 s1 h1 c2 s2 h2 (norm v).
 
-  Module SemanticsExamples.
+Module SemanticsExamples.
 
-    Definition f1 : flow := ens (fun r => pure (r=1)).
-    Definition f2 : flow := req (fun s h => s "x" = Some 1).
+  Definition f1 : flow := ens (fun r => pure (r=1)).
+  Definition f2 : flow := req (fun s h => s "x" = Some 1).
 
-    (* ex z; req x->z; ens[r] x->1/\r=1 *)
-    Definition f3 : flow :=
-      fexists "z" (req (pts "x" "z") ;; ens (fun r => (r=1) //\\ ptsval "x" 1)).
+  (* ex z; req x->z; ens[r] x->1/\r=1 *)
+  Definition f3 : flow :=
+    fexists "z" (req (pts "x" "z") ;; ens (fun r => (r=1) //\\ ptsval "x" 1)).
 
-    Example ex_sem_f1:
-      f1 true sempty hempty true sempty hempty (norm 1).
-      (* sem[true, sempty, hempty]=>[true, sempty, hempty, norm(1)] |= f1. *)
-    Proof.
-      unfold f1.
-      unfold ens.
+  Example ex_sem_f1:
+    f1 true sempty hempty true sempty hempty (norm 1).
+    (* sem[true, sempty, hempty]=>[true, sempty, hempty, norm(1)] |= f1. *)
+  Proof.
+    unfold f1.
+    unfold ens.
+    intuition auto.
+    exists 1.
+    intuition.
+    exists hempty.
+    heap.
+    unfold pure.
+    intuition auto.
+  Qed.
+
+  Example ex_sem_f3:
+    f3 true (supdate "x" 2 sempty) (hupdate 2 3 hempty) 
+      true (supdate "z" 3 (supdate "x" 2 sempty)) (hupdate 2 1 hempty) (norm 1).
+  Proof.
+    unfold f3.
+    unfold fexists.
+    intuition auto.
+    exists 3. (* the initial value of z in ex z. x->z, which is given *)
+    unfold seq.
+    intuition auto.
+    exists (supdate "z" 3 (supdate "x" 2 sempty)).
+    exists hempty.
+    exists (norm 5). (* ret of req, can be anything *)
+    split.
+    - unfold req.
+      intuition auto.
+      exists (hupdate 2 3 hempty).
+      heap.
+      unfold pts.
+      unfold contains.
+      rewrite supdate_other; try congruence.
+      rewrite supdate_same.
+      rewrite supdate_same.
+      eauto.
+    - unfold ens.
       intuition auto.
       exists 1.
-      intuition.
-      exists hempty.
+      intuition auto.
+      exists (hupdate 2 1 hempty).
       heap.
-      unfold pure.
+      unfold pureconj.
       intuition auto.
-    Qed.
+      unfold ptsval.
+      unfold contains.
+      rewrite supdate_other; try congruence.
+      rewrite supdate_same.
+      eauto.
+  Qed.
 
-    Example ex_sem_f3:
-      f3 true (supdate "x" 2 sempty) (hupdate 2 3 hempty) 
-        true (supdate "z" 3 (supdate "x" 2 sempty)) (hupdate 2 1 hempty) (norm 1).
-    Proof.
-      unfold f3.
-      unfold fexists.
-      intuition auto.
-      exists 3. (* the initial value of z in ex z. x->z, which is given *)
-      unfold seq.
-      intuition auto.
-      exists (supdate "z" 3 (supdate "x" 2 sempty)).
-      exists hempty.
-      exists (norm 5). (* ret of req, can be anything *)
-      split.
-      - unfold req.
-        intuition auto.
-        exists (hupdate 2 3 hempty).
-        heap.
-        unfold pts.
-        unfold contains.
-        rewrite supdate_other; try congruence.
-        rewrite supdate_same.
-        rewrite supdate_same.
-        eauto.
-      - unfold ens.
-        intuition auto.
-        exists 1.
-        intuition auto.
-        exists (hupdate 2 1 hempty).
-        heap.
-        unfold pureconj.
-        intuition auto.
-        unfold ptsval.
-        unfold contains.
-        rewrite supdate_other; try congruence.
-        rewrite supdate_same.
-        eauto.
-    Qed.
-
-  End SemanticsExamples.
+End SemanticsExamples.
 
 (* End StagesShallow. *)
 
-    (* forward rules say how to produce a staged formula from a program *)
-    Inductive forward : expr -> flow -> Prop :=
-      | fw_const: forall n,
-        forward (pconst n) (ens (fun res => (res = n) //\\ emp))
+  (* forward rules say how to produce a staged formula from a program *)
+  Inductive forward : expr -> flow -> Prop :=
+    | fw_const: forall n,
+      forward (pconst n) (ens (fun res => (res = n) //\\ emp))
 
-      | fw_var: forall x v,
-        forward (pvar x) (ens (fun res s h => s x = Some v /\ res = v /\ emp s h))
+    | fw_var: forall x v,
+      forward (pvar x) (ens (fun res s h => s x = Some v /\ res = v /\ emp s h))
 
-      (* | fw_deref: forall x y,
-        forward (pderef x) (fexists y (req (pts x y);;
-          ens (fun res s h => ((res = s y) //\\ pts x y) s h)))
+    (* | fw_deref: forall x y,
+      forward (pderef x) (fexists y (req (pts x y);;
+        ens (fun res s h => ((res = s y) //\\ pts x y) s h)))
 
-      | fw_ref: forall x y,
-        (* forward (pref x) (fexists (fun y => ens (fun r s h => contains y (s x) s h))) *)
-        forward (pref x) (fexists y (ens (fun r s h => (r = s y) /\ (pts y x s h)))) *)
+    | fw_ref: forall x y,
+      (* forward (pref x) (fexists (fun y => ens (fun r s h => contains y (s x) s h))) *)
+      forward (pref x) (fexists y (ens (fun r s h => (r = s y) /\ (pts y x s h)))) *)
 
-      | fw_let: forall x e1 e2 f1 f2 f3,
-        forward e1 f1 ->
-        forward e2 f2 ->
-        replace_ret x f1 = f3 ->
-        forward (plet x e1 e2) (fexists x (f3 ;; f2))
+    | fw_let: forall x e1 e2 f1 f2 f3,
+      forward e1 f1 ->
+      forward e2 f2 ->
+      replace_ret x f1 = f3 ->
+      forward (plet x e1 e2) (fexists x (f3 ;; f2))
 
-      (* | fw_get: forall l v, 
-        forward (GET l)
-          (req (contains l v) ;;
-          (ens (fun r => (r = v) //\\ contains l v))) *)
-    .
+    (* | fw_get: forall l v, 
+      forward (GET l)
+        (req (contains l v) ;;
+        (ens (fun r => (r = v) //\\ contains l v))) *)
+  .
 
-  Module ForwardExamples.
+Module ForwardExamples.
 
-    (* let x = 1 in x *)
-    Example ex_forward_let1:
-      exists st, forward (plet "x" (pconst 1) (pvar "x")) st.
-    Proof.
-      eexists.
-      eapply fw_let.
-      eapply fw_const.
-      eapply fw_var.
-      eauto.
-      Unshelve.
-      exact 3. (* anything is allowed it seems *)
-    Qed.
+  (* let x = 1 in x *)
+  Example ex_forward_let1:
+    exists st, forward (plet "x" (pconst 1) (pvar "x")) st.
+  Proof.
+    eexists.
+    eapply fw_let.
+    eapply fw_const.
+    eapply fw_var.
+    eauto.
+    Unshelve.
+    exact 3. (* anything is allowed it seems *)
+  Qed.
 
-    (* Check ex_intro. *)
-    (* ex_intro : forall (A : Type) (P : A -> Prop) (x : A), P x -> exists y, P y *)
-    (* Print ex_forward_let1. *)
-      (* (fun st : ...) is P *)
-      (* (fexists "x" ...) is the witness x, which is what we are after *)
-      (* (fw_let "x" ...) is the existential stmt P x, which is a derivation using the rules above, whose type includes the witness *)
+  (* Check ex_intro. *)
+  (* ex_intro : forall (A : Type) (P : A -> Prop) (x : A), P x -> exists y, P y *)
+  (* Print ex_forward_let1. *)
+    (* (fun st : ...) is P *)
+    (* (fexists "x" ...) is the witness x, which is what we are after *)
+    (* (fw_let "x" ...) is the existential stmt P x, which is a derivation using the rules above, whose type includes the witness *)
 
-  End ForwardExamples.
+End ForwardExamples.
 
 Definition compatible r1 r2 :=
-  match (r1, r2) with
-  | (norm r3, enorm r4) => r3 = r4
-  end.
+match (r1, r2) with
+| (norm r3, enorm r4) => r3 = r4
+end.
 
 Definition wellformed (f:flow) c1 s1 h1 c2 s2 h2 r :=
-  f c1 s1 h1 c2 s2 h2 r -> substore s1 s2.
+f c1 s1 h1 c2 s2 h2 r -> substore s1 s2.
 
 Lemma replace_ret_wellformed : forall x f c1 s1 h1 c2 s2 h2 v,
-  Some v = s1 x ->
-  wellformed f c1 s1 h1 c2 s2 h2 (norm v) ->
-  (wellformed (replace_ret x f)) c1 s1 h1 c2 s2 h2 (norm v).
+Some v = s1 x ->
+wellformed f c1 s1 h1 c2 s2 h2 (norm v) ->
+(wellformed (replace_ret x f)) c1 s1 h1 c2 s2 h2 (norm v).
 Proof.
-  unfold wellformed.
-  intros.
-  unfold replace_ret in H1; destr H1.
-  apply H0.
-  congruence.
+unfold wellformed.
+intros.
+unfold replace_ret in H1; destr H1.
+apply H0.
+congruence.
 Qed.
 
 (* we could prove _wellformed lemmas for all req, ens, etc., but currently we're doing it only for the structures generated from the forward rules *)
 
 Lemma forward_wellformed : forall e f c1 s1 h1 c2 s2 h2 r,
-  forward e f -> (wellformed f) c1 s1 h1 c2 s2 h2 r.
+forward e f -> (wellformed f) c1 s1 h1 c2 s2 h2 r.
 Proof.
-  intros e f c1 s1 h1 c2 s2 h2 r H.
-  revert c1 s1 h1 c2 s2 h2 r.
-  induction H; intros.
-  - unfold wellformed; intros.
-    unfold ens in H; destr H; subst.
-    apply substore_refl.
-  - unfold wellformed; intros.
-    unfold ens in H; destr H; subst.
-    apply substore_refl.
-  -
-    unfold wellformed; intros.
-    unfold fexists in H2; destruct H2 as [? [? [? [v ?]]]]; subst.
-    unfold seq in H5; destruct H5 as [_ [_ [s3 [h3 [? [Hrr Hf2]]]]]]. subst.
+intros e f c1 s1 h1 c2 s2 h2 r H.
+revert c1 s1 h1 c2 s2 h2 r.
+induction H; intros.
+- unfold wellformed; intros.
+  unfold ens in H; destr H; subst.
+  apply substore_refl.
+- unfold wellformed; intros.
+  unfold ens in H; destr H; subst.
+  apply substore_refl.
+-
+  unfold wellformed; intros.
+  unfold fexists in H2; destruct H2 as [? [? [? [v ?]]]]; subst.
+  unfold seq in H5; destruct H5 as [_ [_ [s3 [h3 [? [Hrr Hf2]]]]]]. subst.
 
-    (* introduce well-formed lemma on replace_ret *)
-    pose proof (replace_ret_wellformed x f1 true (supdate x v s1) h1 true s3 h3 v) as Hret.
-    rewrite supdate_same in Hret.
-    assert (Some v = Some v) as triv. reflexivity.
-    specialize (Hret triv); clear triv.
+  (* introduce well-formed lemma on replace_ret *)
+  pose proof (replace_ret_wellformed x f1 true (supdate x v s1) h1 true s3 h3 v) as Hret.
+  rewrite supdate_same in Hret.
+  assert (Some v = Some v) as triv. reflexivity.
+  specialize (Hret triv); clear triv.
 
-    (* assuming f1 is wf using the IH, replace_ret f1 is wf *)
-    specialize (IHforward1 true (supdate x v s1) h1 true s3 h3 (norm v)).
-    specialize (Hret IHforward1).
-    unfold wellformed in Hret.
-    specialize (Hret Hrr).
+  (* assuming f1 is wf using the IH, replace_ret f1 is wf *)
+  specialize (IHforward1 true (supdate x v s1) h1 true s3 h3 (norm v)).
+  specialize (Hret IHforward1).
+  unfold wellformed in Hret.
+  specialize (Hret Hrr).
 
-    unfold wellformed in IHforward2.
-    specialize (IHforward2 true s3 h3 true s2 h2 r Hf2).
+  unfold wellformed in IHforward2.
+  specialize (IHforward2 true s3 h3 true s2 h2 r Hf2).
 
-    unfold wellformed in IHforward1.
-    unfold replace_ret in Hrr; destruct Hrr as [? [? Hf1]]; rewrite supdate_same in H1; inj H1.
-    specialize (IHforward1 Hf1).
-    assert (substore s1 (supdate x v s1)).
-    apply substore_extension; ok.
-    apply substore_trans with (s2 := supdate x v s1); ok.
-    apply substore_trans with (s2 := s3); ok.
+  unfold wellformed in IHforward1.
+  unfold replace_ret in Hrr; destruct Hrr as [? [? Hf1]]; rewrite supdate_same in H1; inj H1.
+  specialize (IHforward1 Hf1).
+  assert (substore s1 (supdate x v s1)).
+  apply substore_extension; ok.
+  apply substore_trans with (s2 := supdate x v s1); ok.
+  apply substore_trans with (s2 := s3); ok.
 Qed.
 
 (* {ens emp} e {\phi}, 
@@ -453,133 +414,131 @@ SH = { (check, s1, h1, R1)   |  [check, S, h] ~~>m [check, s1, h2, R1] |= \phi }
 [S, h, e] -----> [S2, h2, R2], R2!=\bot, 
 such that: 
 \exists (check, s3, h3, R3) \in SH, s3 \subset s2, h3 \subset h2, R2=R1 *)
-    Theorem soundness :
-    forall se1 he1 e se2 he2 re (**) f ss1 hs1 ss2 hs2 rs,
-      bigstep se1 he1 e se2 he2 re ->
-      substore se1 ss1 ->
-      (* he1 = hs1 -> *)
-      forward e f ->
-      f true ss1 hs1 true ss2 hs2 rs ->
-      substore se2 ss2
-      (* /\ he2 = hs2 *)
-      /\ compatible rs re.
-    Proof.
-      intros se1 he1 e se2 he2 re
-             f ss1 hs1 ss2 hs2 rs
-             Hb.
-      revert f ss1 hs1 ss2 hs2 rs.
-      induction Hb;
-      intros f ss1 hs1 ss2 hs2 rs;
-      intros Hsub Hf Hs.
-      - (* var. the proof comes down to the fact that both spec and program read
-           s(x) and leave the heap unchanged. *)
-        inv Hf.
-        unfold ens in Hs; destr Hs.
-        subst.
-        unfold emp in H11.
-        unfold compatible.
-        heap.
-        unfold substore in Hsub.
-        symmetry in H.
-        specialize (Hsub v x H).
-        congruence.
-      -
-        inv Hf.
-        unfold ens in Hs; destr Hs; subst.
-        unfold compatible.
-        unfold pureconj in H8.
-        intuition auto.
-
-      -
-      (* we have an IH for each subexpr *)
-      (* v is the intermediate result of evaluating e1 *)
-      (* r is the final result *)
-      (* invp Hf [H2 H4]. *)
+  Theorem soundness :
+  forall se1 he1 e se2 he2 re (**) f ss1 hs1 ss2 hs2 rs,
+    bigstep se1 he1 e se2 he2 re ->
+    substore se1 ss1 ->
+    (* he1 = hs1 -> *)
+    forward e f ->
+    f true ss1 hs1 true ss2 hs2 rs ->
+    substore se2 ss2
+    (* /\ he2 = hs2 *)
+    /\ compatible rs re.
+  Proof.
+    intros se1 he1 e se2 he2 re
+            f ss1 hs1 ss2 hs2 rs
+            Hb.
+    revert f ss1 hs1 ss2 hs2 rs.
+    induction Hb;
+    intros f ss1 hs1 ss2 hs2 rs;
+    intros Hsub Hf Hs.
+    - (* var. the proof comes down to the fact that both spec and program read
+          s(x) and leave the heap unchanged. *)
       inv Hf.
-      (* invp Hf [ | |Hff1 Hff2]. *)
-      (* inversion Hf as [ Hy Hz |  |Hff1 Hff2 Hz]. subst; clear Hf. *)
-      (* the spec is of the form ex x. f1[x/r];f2 *)
-      unfold fexists in Hs; destruct Hs as [_ [_ [Hnotin [v1 Hseq]]]].
-      (* see how it evaluates *)
-      unfold seq in Hseq; destruct Hseq as [_ [_ [s3 [h3 [? [Hrr ?]]]]]].
-      unfold replace_ret in Hrr; destruct Hrr as [H10 [H9 H13]].
+      unfold ens in Hs; destr Hs.
+      subst.
+      unfold emp in H11.
+      unfold compatible.
+      heap.
+      unfold substore in Hsub.
+      symmetry in H.
+      specialize (Hsub v x H).
+      congruence.
+    -
+      inv Hf.
+      unfold ens in Hs; destr Hs; subst.
+      unfold compatible.
+      unfold pureconj in H8.
+      intuition auto.
+
+    -
+    (* we have an IH for each subexpr *)
+    (* v is the intermediate result of evaluating e1 *)
+    (* r is the final result *)
+    (* invp Hf [H2 H4]. *)
+    inv Hf.
+    (* invp Hf [ | |Hff1 Hff2]. *)
+    (* inversion Hf as [ Hy Hz |  |Hff1 Hff2 Hz]. subst; clear Hf. *)
+    (* the spec is of the form ex x. f1[x/r];f2 *)
+    unfold fexists in Hs; destruct Hs as [_ [_ [Hnotin [v1 Hseq]]]].
+    (* see how it evaluates *)
+    unfold seq in Hseq; destruct Hseq as [_ [_ [s3 [h3 [? [Hrr ?]]]]]].
+    unfold replace_ret in Hrr; destruct Hrr as [H10 [H9 H13]].
 
 
-      (* OLD NOW FIXED now the problem is the IH requires the eval of e1 to take place in the initial stack. but due to the existential adding something to the stack, the evaluation takes place in an extended stack, so we can't apply the IH for e1 *)
+    (* OLD NOW FIXED now the problem is the IH requires the eval of e1 to take place in the initial stack. but due to the existential adding something to the stack, the evaluation takes place in an extended stack, so we can't apply the IH for e1 *)
 
-      (* OLD NOW FIXED the problem is the positioning of the existential has changed. in the program, it's in the e2 initial stack. in the spec, it's right at the front, in the e1 initial stack, for f1 to assign its ret value to. so somehow need to generalise it, using compiler simulation techniques? there should be an initial relation too, so the spec is allowed to execute in an extended stack. so there's a sim rel between configurations *)
+    (* OLD NOW FIXED the problem is the positioning of the existential has changed. in the program, it's in the e2 initial stack. in the spec, it's right at the front, in the e1 initial stack, for f1 to assign its ret value to. so somehow need to generalise it, using compiler simulation techniques? there should be an initial relation too, so the spec is allowed to execute in an extended stack. so there's a sim rel between configurations *)
 
-      (* try to meet in the middle *)
-      (* apply IHHb2. *)
-      (* with (f:=f2) (ss2:=s2) (ss1:=s2) (hs1:=hs2). *)
-      (* easy. *)
-      (* specialize (IHHb1 f1 (supdate x v s) hs1 s1 h1 (norm v) ). *)
-      pose proof (substore_extension_trans _ s ss1 v1 x Hsub Hnotin) as Hha.
-      specialize (IHHb1 f1 (supdate x v1 ss1) hs1 s3 h3 (norm H10) Hha H2 H13).
-      destruct IHHb1 as [IH1 IH2].
-      (* we know that evaluation of e1 preserves substore *)
+    (* try to meet in the middle *)
+    (* apply IHHb2. *)
+    (* with (f:=f2) (ss2:=s2) (ss1:=s2) (hs1:=hs2). *)
+    (* easy. *)
+    (* specialize (IHHb1 f1 (supdate x v s) hs1 s1 h1 (norm v) ). *)
+    pose proof (substore_extension_trans _ s ss1 v1 x Hsub Hnotin) as Hha.
+    specialize (IHHb1 f1 (supdate x v1 ss1) hs1 s3 h3 (norm H10) Hha H2 H13).
+    destruct IHHb1 as [IH1 IH2].
+    (* we know that evaluation of e1 preserves substore *)
 
-      (* now try to use IH2 *)
-      specialize (IHHb2 f2 s3 h3 ss2 hs2 rs).
-      apply IHHb2; auto.
-      apply (substore_extension_left _ s1 s3 v x IH1).
-      unfold compatible in IH2.
-      rewrite <- IH2.
-      rewrite H9.
-      rewrite supdate_same in H9.
-      rewrite supdate_same.
-      (* need to know substore (supdate x v1 ss1) H6 is preserved by all spec/f eval *)
-      (* but how to know that, as we can give any f *)
-      pose proof (forward_wellformed _ _ true (supdate x v1 ss1) hs1 true s3 h3 (norm H10) H2) as Hf1wf.
-      unfold wellformed in Hf1wf.
+    (* now try to use IH2 *)
+    specialize (IHHb2 f2 s3 h3 ss2 hs2 rs).
+    apply IHHb2; auto.
+    apply (substore_extension_left _ s1 s3 v x IH1).
+    unfold compatible in IH2.
+    rewrite <- IH2.
+    rewrite H9.
+    rewrite supdate_same in H9.
+    rewrite supdate_same.
+    (* need to know substore (supdate x v1 ss1) H6 is preserved by all spec/f eval *)
+    (* but how to know that, as we can give any f *)
+    pose proof (forward_wellformed _ _ true (supdate x v1 ss1) hs1 true s3 h3 (norm H10) H2) as Hf1wf.
+    unfold wellformed in Hf1wf.
 
-      (* assert (Hpreserve : substore (supdate x v1 ss1) s3). admit. *)
-      (* apply Hf1wf. *)
-      (* unfold substore in Hpreserve. *)
-      (* apply Hpreserve. *)
-      apply Hf1wf.
-      ok.
-      rewrite supdate_same.
-      reflexivity.
+    (* assert (Hpreserve : substore (supdate x v1 ss1) s3). admit. *)
+    (* apply Hf1wf. *)
+    (* unfold substore in Hpreserve. *)
+    (* apply Hpreserve. *)
+    apply Hf1wf.
+    ok.
+    rewrite supdate_same.
+    reflexivity.
 
 (* https://xavierleroy.org/courses/EUTypes-2019/slides.pdf *)
 
-    Qed.
+  Qed.
 
-  (* Module SpecExamples.
-    Example ex_spec_return_anything: exists x,
-      sem[ true, sempty, hempty]=>[ true, sempty, hempty, norm x] |= req emp.
-    Proof.
-      exists 1.
-      apply sem_req with (s1 := sempty).
-      auto.
-      exists hempty.
-      repeat split; heap.
-    Qed.
+(* Module SpecExamples.
+  Example ex_spec_return_anything: exists x,
+    sem[ true, sempty, hempty]=>[ true, sempty, hempty, norm x] |= req emp.
+  Proof.
+    exists 1.
+    apply sem_req with (s1 := sempty).
+    auto.
+    exists hempty.
+    repeat split; heap.
+  Qed.
 
-    Example ex_spec_ens_1:
-      sem[ true, sempty, hempty]=>[ true, sempty, hempty, norm 1] |=
-        ens (fun r => (r = 1) //\\ emp).
-    Proof.
-      apply sem_ens with (s := sempty).
-      exists hempty.
-      repeat split; heap.
-    Qed.
+  Example ex_spec_ens_1:
+    sem[ true, sempty, hempty]=>[ true, sempty, hempty, norm 1] |=
+      ens (fun r => (r = 1) //\\ emp).
+  Proof.
+    apply sem_ens with (s := sempty).
+    exists hempty.
+    repeat split; heap.
+  Qed.
 
-    Example ex_spec_seq: forall x,
-      sem[ true, sempty, hupdate x 1 hempty]=>[ true, sempty, hupdate x 1 hempty, norm 2] |= (req (contains x 1);; ens (fun r => (r = 2) //\\ contains x 1)).
-    Proof.
-      intros.
-      apply sem_seq with (s1 := sempty) (h2 := hempty) (r := norm 3).
-      - apply sem_req with (s1 := sempty).
-      exists (hupdate x 1 hempty).
-      repeat split.
-      heap.
-      heap.
-      - apply sem_ens with (s := sempty).
-      exists (hupdate x 1 hempty).
-      repeat split; heap.
-    Qed.
-  End SpecExamples. *)
-
-End Flow3.
+  Example ex_spec_seq: forall x,
+    sem[ true, sempty, hupdate x 1 hempty]=>[ true, sempty, hupdate x 1 hempty, norm 2] |= (req (contains x 1);; ens (fun r => (r = 2) //\\ contains x 1)).
+  Proof.
+    intros.
+    apply sem_seq with (s1 := sempty) (h2 := hempty) (r := norm 3).
+    - apply sem_req with (s1 := sempty).
+    exists (hupdate x 1 hempty).
+    repeat split.
+    heap.
+    heap.
+    - apply sem_ens with (s := sempty).
+    exists (hupdate x 1 hempty).
+    repeat split; heap.
+  Qed.
+End SpecExamples. *)
