Biabduction.v
@@ -1,0 +1,41 @@
+
+From Coq Require Import ZArith Lia Bool List String Program.Equality.
+From Coq Require Import FunctionalExtensionality PropExtensionality.
+From CDF Require Import Common Sequences Separation2 Tactics.
+
+Local Open Scope string_scope.
+(* Local Open Scope nat_scope. *)
+Local Open Scope Z_scope.
+Local Open Scope list_scope.
+
+(* like the member predicate. or modulo equivalence? *)
+Inductive split : assertion -> assertion -> assertion -> Prop :=
+  | split_one : forall h2 x y,
+    split (pts x y ** h2) (pts x y) h2
+
+  | split_next : forall h2 x y h h1,
+    split h1 h h2 ->
+    split (pts x y ** h2) h h2
+.
+
+Inductive biab : assertion -> assertion -> assertion -> Prop :=
+
+  | biab_base : forall s m,
+    biab s m (pure True)
+
+  | biab_missing : forall x y a m,
+    biab emp ((pts x y) ** m) ((pts x y) ** a)
+
+  | biab_match : forall x y z a b m m1,
+    biab b m a ->
+    (z = y) //\\ m = m1 ->
+    biab ((pts x z) ** b) m1 ((pts x y) ** a)
+.
+
+Example ex1 : forall x y a b,
+  biab (pts x y ** emp) (pts a b) (pts x y ** pts a b).
+Proof.
+  intros.
+  apply biab_match with (m := pts a b).
+  (* apply biab_missing with (m := pts a b). *)
+Admitted.
